Add pi type

syntax.sig
@@ -7,3 +7,4 @@ Abs : (bind Tm in Tm) -> Tm
 App : Tm -> Tm -> Tm
 Pair : Tm -> Tm -> Tm
 Proj : PTag -> Tm -> Tm
+Pi : Tm -> (bind Tm in Tm) -> Tm
